\usepackage[utf8]{inputenc}
\documentclass[12pt]{article}
\usepackage{amsmath}
\usepackage{amssymb}
\usepackage{amsthm}
\usepackage{amsfonts}
\usepackage{graphicx} 

\title{HW2 - CS006}
\author{Rafael Betita}
\date{March 2019}

\begin{document}

\maketitle

\newpage

\begin{enumerate}
    \item \text{Prove the following theorems algebraically:}
    \begin{enumerate}
        \item 
            \begin{align*}
            X(X'+Y)&=XY\\
            XX'+XY&=XY\\
            0+XY&=XY
            \end{align*}
        \item
            \begin{align*}
                X+XY&=X\\
                X(1+Y)&=X\\
                X(1)&=X
            \end{align*}
        \item
            \begin{align*}
                XY+XY'&=X\\
                X(Y+Y')&=X\\
                X(1)&=X
            \end{align*}
        \item
            \begin{align*}
                (A+B)(A+B')&=A\\
                AA+AB'+BA+BB'&=A\\
                A+AB'+AB&=A\\
                A+A(B+B')&=A\\
                A+A&=A\\
                A&=A
            \end{align*}
    \end{enumerate}
    \newpage\addtocounter{enumi}{1}\item Simplify each of the following expressions by applying one of the theorems. State the theorem used.
        \begin{enumerate}
            \item X'Y'Z+(X'Y'Z)' = 1 
            \\\text{Uniting Theorems}\\
            \item (AB'+CD)(B'E+CD) = CD+AB'B'E = CD+AB'E
            \\\text{Distributive Laws}\\
            \item (ACF+AC'F) = AF
            \\\text{Uniting Theorem}\\
            \item A(C+D'B)+A' = A'+(C+D'B)
            \\\text{Elimination Theorem}\\
            \item (A'B+C+D)(A'B+D) = A'B+D
            \\\text{Absorption Theorem}\\
            
            \item (A+BC)+(DE+F)(A+BC)'=(A+BC)+(DE+F)
            \\\text{Elmination Theorem}
        \end{enumerate}
    \addtocounter{enumi}{1}\item Multiply out and simplify to obtain a sum of products:
        \begin{enumerate}
            \item (A+B)(C+B)(D'+B)(ACD'+E)
            \begin{align*}
                (AC+B)(D'+B)(ACD'+E) && \text{Distributive Law}\\
                (B+ACD')(ACD'+E)&& \text{Distributive Law}\\
                BE+ACD' && \text{Distributive Law}
            \end{align*}
            \item  (A'+B+C')(A'+C'+D)(B'+D')
            \begin{align*}
                (A'+C'+BD)(B'+D') && \text{Distributive Law}\\
                A'B'+A'D'+C'B'+C'D'+BB'D+BDD'\\
                A'B'+A'D'+C'B'+C'D'\\
            \end{align*}
        \end{enumerate}
    \newpage\addtocounter{enumi}{1}\item Draw a circuit that uses only one AND gate and one OR gate to realize each of the following functions:
        \begin{enumerate}
            \item (A+B+C+D)(A+B+C+E)(A+B+C+F) = (A+B+C+DEF)
            \item (WXYZ+VXYZ+UXYZ) = XYZ(W+V+U)
        \end{enumerate}
    \addtocounter{enumi}{1}\item Find F and G and simplify
    \begin{enumerate}
        \item F = ((A+B)'+((A+(A+B)')')((A+(A+B)')')
        \begin{align*}
            (A+(A+B)')' &\text{ Absorption Theorem}\\
            (A+A'B')' &\text{ DeMorgan's Law}\\
            (A+B')' = A'B &\text{ DeMorgan's Law}
        \end{align*}
        \item G = (((R+S+T)'(P)((R+S)'(T)))'(T))'
        \begin{align*}
            (R+S+T)'(PT)(R+S)'+T' &\text{ DeMorgan's Law}\\
            (R+S+T)'(PT)(R+S)'+T' &\text{ DeMorgan's Law}\\            (R'S'T')(PT)(R'S')+T' &\text{ DeMorgan's Law}\\
            0+T' = T'
        \end{align*}
    \end{enumerate}
    \addtocounter{enumi}{1}\item Simplify each of the following expressions by applying one of the theorems. State the theorem used.
    \begin{enumerate}
        \item (A'+B'+C)(A'+B'+C)' = 0\\\text{Complementarity Law}
        \item AB(C'+D)+B(C'+D) = B(C'+D)\\\text{ Absorption Theorem}
        \item AB+(C'+D)(AB)' = AB+(C'+D)\\\text{ Elimination Theorem}
        \item (A'BF+CD')(A'BF+CEG) = A'BF+CEGCD' = A'BF+CEGD'\\\text{ Elimination Theorem}
        \item ([AB'+(C+D)'+E'F](C+D)) = AB'(C+D)+0+E'F(C+D)
        \\\text{Distributive Law}
        \item A'(B+C)(D'E+F)'+(D'E+F) = (D'E+F)+A'(B+C)
        \\\text{ Elimination Theorem}
    \end{enumerate}
    \newpage\addtocounter{enumi}{1}\item
    \begin{enumerate}
        \item 
        \begin{align*}
         F_1&=A'A+B+(B+B)\\
         &=B
        \end{align*}
        \item
        \begin{align*}
            F_2 &= A'A'+AB'\\
            &= A'+AB'\\
            &= A'+B'
        \end{align*}
        \item
        \begin{align*}
            F_3 &= ((AB+C)'D)((AB+C)+D)\\
            &= ((AB+C)'D)(AB+C)+D((AB+C)'D)\\
            &= ((AB+C)'D)
        \end{align*}
        \item
        \begin{align*}
            Z &=((A+B)C)'+(A+B)CD\\
            &= ((A+B)C)' + D\\
            &= (A+B)'+C'+D\\
            &= A'B'+C'+D
        \end{align*}
    \end{enumerate}
    \addtocounter{enumi}{1}\item Use only DeMorgan's relationships and Involution to find the complements of the following functions:
    \begin{enumerate}
        \item f(A,B,C,D) = [A+(BCD)'][(AD)'+B(C'+A)]
        \begin{align*}
            f' &= [A+B'+C'+D']'+[(A'+D')+B(C'+A)]'\\
            &= A'BCD+(A'+D')'(B(C'+A))'\\
            &= A'BCD+(AD)(B'+(C'+A)')\\
            &= A'BCD+(AD)(B'+CA')\\
            &= A'BCD+AB'D
        \end{align*}
        \item f(A,B,C,D) = AB'C+(A'+B+D)(ABD'+B')
        \begin{align*}
            f' &=  (AB'C+(A'+B+D)(ABD'+B'))'\\
            &=  ((AB'C)'((A'+B+D)(ABD'+B'))')\\
            &=  ((A'+B''+C')((A'+B+D)'+(ABD'+B')'))\\
            &=  ((A'+B+C')((A''B'+D')+((ABD')'(B''))))\\
            &=  ((A'+B+C')((A''B'+D')+((A'+B'+D)(B)))\\
        \end{align*}
    \end{enumerate}
      \addtocounter{enumi}{1}\item For the following switching circuit, find the logic function expression describing the circuit by the three methods indicated, simplify each expression and show they are equal. 
\end{enumerate}

\end{document}
